ProgTheorems.v
@@ -1,0 +1,39 @@
+Require Import Automation.
+Require Import Prog.
+Require Import ProofIrrelevance.
+
+(** Here we prove some basic sanity checks on prog and its semantics. *)
+
+Hint Constructors exec.
+
+Theorem can_crash_at_begin : forall T (p: prog T) sigma,
+    exec p sigma (Crashed sigma).
+Proof.
+  eauto.
+Qed.
+
+Ltac inj_pair2 :=
+  match goal with
+  | [ H: existT ?P ?A _ = existT ?P ?A _ |- _ ] =>
+    apply inj_pair2 in H; subst
+  end.
+
+Ltac inv_exec :=
+  match goal with
+  | [ H: exec _ _ _ |- _ ] =>
+    inversion H; subst; clear H;
+    repeat inj_pair2
+  end.
+
+Theorem can_crash_at_end : forall T (p: prog T) sigma v sigma',
+    exec p sigma (Finished v sigma') ->
+    exec p sigma (Crashed sigma').
+Proof.
+  induction p; intros;
+    inv_exec;
+    eauto.
+Qed.
+
+(* Local Variables: *)
+(* company-coq-local-symbols: (("Sigma" . ?Σ) ("sigma" . ?σ) ("sigma'" . (?σ (Br . Bl) ?'))) *)
+(* End: *)
